{
 "cells": [
  {
   "cell_type": "markdown",
   "metadata": {},
   "source": [
    "**A. Determine whether the ff. are convergent or divergent. (5 pts. each)**\n",
    "\n",
    "1. $A = \\left\\langle \\frac{n^2 - 4}{\\sqrt{n^4 + 4n^2 + 4}} \\right\\rangle$\n",
    "\n",
    "    $$\n",
    "    \\begin{align}\n",
    "    \\frac{n^2 - 4}{\\sqrt{n^4 + 4n^2 + 4}} & = \\frac{n^2 - 4}{n^2 \\sqrt{1 + \\frac{4}{n^2} + \\frac{4}{n^4}}} \\\\\n",
    "    & = \\frac{1 - \\frac{4}{n^2}}{\\sqrt{1 + \\frac{4}{n^2} + \\frac{4}{n^4}}} \\\\\n",
    "    & \\to \\frac{1 - 0}{\\sqrt{1 + 0 + 0}} = \\frac{1}{1} = 1 & \\therefore \\text{convergent}\n",
    "    \\end{align}\n",
    "    $$\n",
    "\n",
    "2. $B = \\left\\langle \\frac{n!}{n^n} \\right\\rangle$\n",
    "\n",
    "    $$\n",
    "    \\begin{align}\n",
    "    \\frac{n!}{n^n} & \\approx \\frac{\\sqrt{2\\pi n} \\left( \\frac{n}{e} \\right)^n}{n^n} & \\text{I would never figure this out alone.}\\\\\n",
    "    & = \\frac{\\sqrt{2\\pi n} \\cdot n^n \\cdot e^{-n}}{n^n} \\\\\n",
    "    & \\to \\sqrt{2\\pi n} \\cdot e^{-n} = 0 & \\therefore \\text{convergent}\n",
    "    \\end{align}\n",
    "    $$\n",
    "\n",
    "3. $C = \\sum \\frac{2n^2}{4n^2 + 2}$\n",
    "\n",
    "    $$\n",
    "    \\begin{align}\n",
    "    a_n & = \\frac{2n^2}{4n^2 + 2} \\\\\n",
    "    & = \\frac{1}{2 + \\frac{1}{n^2}} \\\\\n",
    "    & \\to \\frac{1}{2 + 0} = \\frac{1}{2} \\neq 0 & \\therefore \\text{divergent}\n",
    "    \\end{align}\n",
    "    $$\n",
    "\n",
    "4. $D = \\sum (-1)^n \\left( \\frac{n}{3n - 2} \\right)$\n",
    "\n",
    "    $$\n",
    "    \\begin{align}\n",
    "    a_n & = \\left| \\frac{n}{3n - 2} \\right| = \\frac{n}{3n - 2} \\\\\n",
    "    & = \\frac{1}{3 - \\frac{2}{n}} \\\\\n",
    "    & \\to \\frac{1}{3 - 0} = \\frac{1}{3} \\neq 0 & \\therefore \\text{divergent}\n",
    "    \\end{align}\n",
    "    $$\n",
    "\n",
    "**B. From items #s (3 - 4), determine whether the ff. are absolutely convergent or conditional convergent (if applicable) (10 pts. each)**\n",
    "\n",
    "5. $C = \\sum \\frac{2n^2}{4n^2 + 2}$ **(not applicable)**\n",
    "6. $D = \\sum (-1)^n \\left( \\frac{n}{3n - 2} \\right)$ **(not applicable)**\n",
    "\n",
    "**C. Find the infimum & supremum of the ff. (6 pts. each)**\n",
    "\n",
    "7. $E = \\left\\{ \\frac{2}{n} + \\frac{4}{m} | n, m \\in \\mathbb{N} \\right\\}$\n",
    "\n",
    "    $$\n",
    "    \\begin{align}\n",
    "    a_{n, m} & = \\frac{2}{n} + \\frac{4}{m} & \\lim_{n, m \\to \\infty} \\left( \\frac{2}{n} + \\frac{2}{m} \\right) & = 0\\\\\n",
    "    a_{1, 1} & = \\frac{2}{1} + \\frac{4}{1} = 6 \\\\\n",
    "    \\therefore \\sup E & = 6 & \\inf E & = 0\n",
    "    \\end{align}\n",
    "    $$\n",
    "\n",
    "8. $F = \\left\\{ \\frac{n!}{n^n} | n \\in \\mathbb{N} \\right\\}$\n",
    "\n",
    "    $$\n",
    "    \\begin{align}\n",
    "    a_n & = \\frac{n!}{n^n} = \\frac{1 \\cdot 2 \\cdot 3 \\cdots n}{n \\cdot n \\cdot n \\cdots n} = \\frac{1}{n} \\cdot \\frac{2}{n} \\cdot \\frac{3}{n} \\cdots \\frac{n}{n} \\\\\n",
    "    & = \\prod_{k = 1}^{n} \\frac{k}{n} \\approx \\frac{\\sqrt{2\\pi n}}{e^n} & \\to & = 0 \\\\\n",
    "    a_1 & = \\frac{1!}{1^1} = \\frac{1}{1} = 1 \\\\\n",
    "    \\therefore \\sup F & = 1 & \\inf F & = 0\n",
    "    \\end{align}\n",
    "    $$\n",
    "\n",
    "**D. Prove the ff. (5 pts)**\n",
    "\n",
    "9. Using PMI, prove that\n",
    "\n",
    "    $$\n",
    "    1^3 + 2 ^3 + 3^3 + \\dots + n^3 = \\left[ \\frac{1}{2} (n (n + 1)) \\right]^2\n",
    "    $$\n",
    "\n",
    "    for all $n \\in \\mathbb{N}$.\n",
    "\n",
    "    **Answer:**\n",
    "\n",
    "    Assume $n = 1$:\n",
    "\n",
    "    $$\n",
    "    1^3 = 1, \\left[ \\frac{1(1 + 1)}{2} \\right]^2 = \\left[ \\frac{1 \\cdot 2}{2} \\right]^2 = 1^2 = 1\\\\\n",
    "    $$\n",
    "\n",
    "    The formula holds for $n = 1$.\n",
    "\n",
    "    Assume that the formula holds for some $n = k$:\n",
    "\n",
    "    $$\n",
    "    1^3 + 2^3 + 3^3 + \\dots + k^3  = \\left[ \\frac{k(k + 1)}{2} \\right]^2\n",
    "    $$\n",
    "\n",
    "    We need to prove that the formula also holds for $n = k + 1$:\n",
    "\n",
    "    $$\n",
    "    1^3 + 2^3 + 3^3 + \\dots + (k + 1)^3 = \\left[ \\frac{(k + 1)(k + 2)}{2} \\right]^2\n",
    "    $$\n",
    "\n",
    "    Using the induction hypothesis:\n",
    "\n",
    "    $$\n",
    "    \\begin{align}\n",
    "    1^3 + 2^3 + 3^3 + \\dots + k^3 + (k + 1)^3 & = \\left[ \\frac{k(k + 1)}{2} \\right]^2 + (k + 1)^3 \\\\\n",
    "    & = \\frac{k^2(k + 1)^2}{4} + {k + 1}^3 \\\\\n",
    "    & = (k + 1)^2 \\left( \\frac{k^2}{4} + (k + 1) \\right) \\\\\n",
    "    & = (k + 1)^2 \\left( \\frac{k^2 + 4(k + 1)}{4} \\right) \\\\\n",
    "    & = (k + 1)^2 \\left( \\frac{k^2 + 4k + 4}{4} \\right) \\\\\n",
    "    & = (k + 1)^2 \\times \\frac{(k + 2)^2}{4} \\\\\n",
    "    & = \\left[ \\frac{(k + 1)(k + 2)}{2} \\right]^2\n",
    "    \\end{align}\n",
    "    $$\n",
    "    \n",
    "    **Therefore**, by using the pinciple of mathematical induction, the formula\n",
    "\n",
    "    $$\n",
    "    1^3 + 2 ^3 + 3^3 + \\dots + n^3 = \\left[ \\frac{1}{2} (n (n + 1)) \\right]^2\n",
    "    $$\n",
    "\n",
    "    holds for all $n \\in \\mathbb{N}$."
   ]
  }
 ],
 "metadata": {
  "language_info": {
   "name": "python"
  }
 },
 "nbformat": 4,
 "nbformat_minor": 2
}
